theories/CTree/Logic/AG.v
@@ -387,25 +387,25 @@ End CtlAgState.
 Section CtlAgW.
   Context {E Σ W: Type} {HE: Encode E} (h:E ~> stateT Σ (ctree void)). 
 
-  Theorem ag_iterW{X I}: forall (σ: Σ) (k: I -> ctree E (I + X)) (i: I) (φ: Σ -> Prop) R,
-      R i ->          (* Iterator invariant [R] *)
-      φ σ ->          (* Initial state precondition [φ] *)
+  Theorem ag_iterW{X I}: forall (σ: Σ) (k: I -> ctree E (I + X)) (i: I) (φ: Σ -> Prop) Ri Rv,
+      Ri i ->         (* Iterator invariant [Ri] *)
+      φ σ ->          (* Goal Invariant [φ] *)
       (forall (x: I) (σ: Σ),
-          R x ->
+          Ri x ->
           φ σ ->
           <( {interp_state (h_writerΣ h) (k x) σ}, {Obs (Log σ) tt} |=
               AX (visW φ AU AX
                     (finishW {fun (lr: I + X) (σ σ': Σ) =>
-                                σ = σ' /\ (* A property of [h_writerΣ h] is it logs σ and then returns it [σ'] *)
-                                exists (i: I), lr = inl i /\ R i /\ φ σ})))>) ->
+                                σ = σ' /\ (* [h_writerΣ h] logs σ, then returns it [σ'] *)
+                                exists (i: I), lr = inl i /\ Ri i /\ φ σ /\ Rv x i})))>) ->
       <( {interp_state (h_writerΣ h) (iter k i) σ}, {Obs (Log σ) tt} |= AG visW φ )>.
   Proof with eauto with ctl.
     setoid_rewrite ctl_vis_now.
     setoid_rewrite ctl_finish_done.
     intros.
     rewrite interp_state_unfold_iter.
-    generalize dependent i.
     generalize dependent σ.
+    generalize dependent i.    
     coinduction RR CIH; intros.
     apply RStepA; [apply ctl_now; eauto with ctl |].
     split.
@@ -435,16 +435,16 @@ Section CtlAgW.
                            '(x0, s) := x in
                             fun pat0 : writerE Σ =>
                             let
-                              'Log v0 as u := pat0 return (encode u -> Prop) in fun 'tt =>
-                                                                              s = v0 /\
-                                                                              exists i : I, x0 = inl i /\ R i /\ φ s)
+                              'Log v0 as u := pat0 return (encode u -> Prop) in
+                            fun 'tt => s = v0 /\
+                                      exists i' : I, x0 = inl i' /\ Ri i' /\ φ s /\ Rv i i')
                             e v))); cbn.
         apply in_bind_ctx1.
         * specialize (H1 _ _ H H0) as HAX.
           cdestruct HAX.
           specialize (HAX _ _ TR0).
           apply HAX.
-        * intros (lr' & s_) w ([σ'] & [] & ? & ? & i' & -> & ? & ?); subst.
+        * intros (lr' & s_) w ([σ'] & [] & ? & ? & i' & -> & ? & ? & ?); subst.
           unfold Classes.iter, MonadIter_ctree.          
           apply (ft_t (mequ_clos_car (KS:=KripkeSetoidSBisim))); cbn.
           econstructor.
